Added the dereferencing lens and number of other bits to UTP memory

theories/memory/utp_mem_prelim.thy
@@ -1,10 +1,15 @@
+section \<open> Memory Preliminaries \<close>
+
 theory utp_mem_prelim
   imports 
     Partial_Monoids
     Partial_Monoids_Instances
-    "UTP-Designs.utp_designs" 
+    "UTP-Undef.utp_undef" 
+    "Continuum.Lightweight_Cardinals"
     "UTP.utp_full"
 begin recall_syntax
+
+subsection \<open> State space \<close>
 
 text \<open> As usual, the memory consists of the store and the heap. The store is an abstract
   type, and will usually be another alphabet. \<close>
@@ -39,7 +44,54 @@ translations
 type_synonym ('h, 's) spred = "('h, 's) mem_ext upred"
 type_synonym ('h, 's) sprog = "('h, 's) mem_ext hrel_des"
 
-type_synonym 's mpred = "((nat, nat) ffun, 's) spred"
-type_synonym 's mprog = "((nat, nat) ffun, 's) sprog"
+text \<open> For now we represent addresses and data as naturals. We can therefore inject
+  countable data structures into our memory model. \<close>
+
+type_synonym addr = nat
+type_synonym data = nat
+
+type_synonym 's mpred = "((addr, data) ffun, 's) spred"
+type_synonym 's mprog = "((addr, data) ffun, 's) sprog"
+type_synonym ('a, 's) mexpr = "('a, ((addr, data) ffun, 's) mem_ext) pexpr"
+
+subsection \<open> Dereferencing Lens \<close>
+
+definition ind_lens :: "('i \<Rightarrow> ('a \<Longrightarrow> 's)) \<Rightarrow> ('i \<Longrightarrow> 's) \<Rightarrow> ('a \<Longrightarrow> 's)" where
+[lens_defs]: "ind_lens f x = \<lparr> lens_get = (\<lambda> s. get\<^bsub>f (get\<^bsub>x\<^esub> s)\<^esub> s), lens_put = (\<lambda> s v. put\<^bsub>f (get\<^bsub>x\<^esub> s)\<^esub> s v) \<rparr>"
+
+lemma ind_lens_mwb [simp]: "\<lbrakk> \<And> i. mwb_lens (F i); \<And> i. (F i) \<bowtie> x \<rbrakk> \<Longrightarrow> mwb_lens (ind_lens F x)"
+  by (unfold_locales, auto simp add: lens_defs lens_indep.lens_put_irr2)
+
+lemma ind_lens_vwb [simp]: "\<lbrakk> \<And> i. vwb_lens (F i); \<And> i. (F i) \<bowtie> x \<rbrakk> \<Longrightarrow> vwb_lens (ind_lens F x)"
+  by (unfold_locales, auto simp add: lens_defs lens_indep.lens_put_irr2)
+
+text \<open> We first create a bijective lens that extracts a countable type from a natural number. \<close>
+
+definition to_nat_lens :: "'a::{countable,infinite} \<Longrightarrow> nat" ("to-nat\<^sub>L") where
+[lens_defs]: "to_nat_lens = \<lparr> lens_get = \<lambda> s. from_nat_bij s, lens_put = \<lambda> s v. to_nat_bij v \<rparr>"
+
+lemma to_nat_lens_bij [simp]: "bij_lens to_nat_lens"
+  by (unfold_locales, simp_all add: lens_defs)
+
+text \<open> The dereferencing lens obtains the heap, applies the finite function lens with the given
+  address, and finally obtains the type data. \<close>
+
+definition deref :: "(addr \<Longrightarrow> 's) \<Rightarrow> ('a::{countable,infinite} \<Longrightarrow> ((nat, nat) ffun, 's) mem_ext)" where
+[lens_defs]: "deref a = to-nat\<^sub>L ;\<^sub>L ind_lens (\<lambda> i. ffun_lens i ;\<^sub>L hp) (a ;\<^sub>L str)"
+
+syntax \<comment> \<open> Dereferencing Variable Identifier \<close>
+  "_spderef"       :: "id \<Rightarrow> svid" ("*_")
+
+translations
+  "_spderef a" == "CONST deref a"
+
+lemma src_deref: "vwb_lens a \<Longrightarrow> \<S>\<^bsub>deref a\<^esub> = {s. get\<^bsub>a ;\<^sub>L str\<^esub> s \<in> fdom(get\<^bsub>hp\<^esub> s)}"
+  apply (simp add: deref_def source_lens_comp wb_lens.source_UNIV ffun_lens_src)
+  apply (auto simp add: lens_defs lens_source_def)
+  apply (metis ffun_upd_ext mem.surjective mem.update_convs(1))
+  done
+
+lemma src_pred_deref: "vwb_lens a \<Longrightarrow> \<^bold>S(deref a) = (&str:a \<in>\<^sub>u dom\<^sub>u(&hp))"
+  by (simp add: src_pred_def src_deref, rel_auto)
 
 end
