theories/undef/utp_undef.thy
@@ -20,7 +20,23 @@ update_uexpr_rep_eq_thms
 lemma undef_defined: "\<D>(\<bottom>\<^sub>\<D>) = false"
   by (rel_simp)
 
+definition src_pred :: "('a \<Longrightarrow> 's) \<Rightarrow> 's upred" ("\<^bold>S'(_')") where
+[upred_defs]: "src_pred x = (&\<^bold>v \<in>\<^sub>u \<guillemotleft>\<S>\<^bsub>x\<^esub>\<guillemotright>)"
+
+lemma wb_lens_src_true [simp]: "wb_lens x \<Longrightarrow> \<^bold>S(x) = true"
+  by (rel_simp, simp add: wb_lens.source_UNIV) 
+
 definition partial_assign :: "('a \<Longrightarrow> '\<alpha>) \<Rightarrow> ('a, '\<alpha>) pexpr \<Rightarrow> '\<alpha> hrel_des" where
-[upred_defs]: "partial_assign x e = (&\<^bold>v \<in>\<^sub>u \<guillemotleft>\<S>\<^bsub>x\<^esub>\<guillemotright> \<and> \<D>(e)) \<turnstile>\<^sub>n x := \<lfloor>e\<rfloor>\<^sub>\<D>"
+[upred_defs]: "partial_assign x e = (\<^bold>S(x) \<and> \<D>(e)) \<turnstile>\<^sub>n x := \<lfloor>e\<rfloor>\<^sub>\<D>"
+
+syntax
+  "_passignd" :: "svid \<Rightarrow> uexp \<Rightarrow> logic"  (infixr ":=\<^sub>\<D>" 62)
+
+translations
+  "_passignd x e" == "CONST partial_assign x e"
+
+lemma passign_bot: "x :=\<^sub>\<D> \<bottom>\<^sub>\<D> = \<bottom>\<^sub>D"
+  by (rel_auto)
+
 
 end
